# 2.4 - 7
$$p(x) = x^2-7x+10 =0$$
$$q(x) = x^2-2x-3 =0$$
$$r(x) < 0$$

### Question a
1) $\forall x[p(x) \rightarrow \neg r(x)] \rightarrow true$
2) $\forall x[q(x) \rightarrow r(x)] \rightarrow counterexample: x = 3$
3) $\exists x[q(x) \rightarrow r(x)] \rightarrow true$
4)  $\exists x[p(x) \rightarrow r(x)] \rightarrow true$

### Question b
1) $\forall x[p(x) \rightarrow \neg r(x)] \rightarrow true$
2) $\forall x[q(x) \rightarrow r(x)] \rightarrow counterexample: x = 3$
3) $\exists x[q(x) \rightarrow r(x)] \rightarrow true$
4)  $\exists x[p(x) \rightarrow r(x)] \rightarrow true$

### Question c
1) $\forall x[p(x) \rightarrow \neg r(x)] \rightarrow true$
2) $\forall x[q(x) \rightarrow r(x)] \rightarrow true$
3) $\exists x[q(x) \rightarrow r(x)] \rightarrow true$
4) $\exists x[p(x) \rightarrow r(x)] \rightarrow false: x = 2 \lor x = 5$

# 2.4 - 10
### Question a) 
$\forall m, n : A[m,n] > 0$

### Question b) 
$\forall m, n : 0 < A[m,n] \leq 70$

### Question c) 
$\exists m, n : A[m,n] > 60$

### Question d) 
$\forall m, [1 \leq n \leq 20] A[m,n] > A(m,n-1)$

### Question e) 
$\forall n, [1 \leq m \leq 20] A[m,n] > A(m-1,n)$

### Question f) 
$???$

# 2.4 - 15
### Question a) 
This statement is true

### Question b) 
The negation is wrong. The correct negation states that for all rational numbers x, y, the sum of x + y is rational as well.

### Question c) 
The original statement is true

### Question d) 
The statement is true, the negation isn't. 


# 2.4 - 23
### Question a) 
$\exists e \forall a [a + z = z + a = 0]$

### Question b) 
$\exists e \forall a [a * z = z * a = a]$

### Question c) 
$\exists e \forall a \neq 0 [a * z = z * a = 1]$

### Question d) 
Statement (b) remains true in the new universe but statement (c) does not.


# 2.4 - 25
### Question a) 
Step | Item
| - | - | 
$\forall x \forall y [(x > y) \rightarrow (x - y > 0)]$ | Original
$\neg(\forall x \neg \forall y [(x > y) \rightarrow (x - y > 0)])$ | Negation
$(\exists x \neg \forall y [\neg(x > y) \rightarrow (x - y > 0)])$ | N1
$(\exists x \exists y [\neg \neg(x > y) \rightarrow (x - y > 0)])$ | N1
$(\exists x \exists y [(x > y) \rightarrow (x - y > 0)])$ | double negation



###  Question b) 
$\forall x \forall y [(x < y) \rightarrow \exists z (x < y < z)]$

### Question c) 
$\forall x \forall y [(|x| = |y|) \rightarrow (y = \plusmn x)]$


# 2.5 - 8



# 2.5 - 9


# 2.5 - 11




