| Law number |    Name of the law     | the law                                                                                                                                          |
| :--------- | :--------------------: | :----------------------------------------------------------------------------------------------------------------------------------------------- |
| L1         | double negotiation Law | $$ \neg \neg p \Leftrightarrow p $$                                                                                                              |
| L2         |     DeMorgan's Law     | $$ \neg (p \vee q) \Leftrightarrow \neg p \wedge \neg q $$  $$ \neg (p \wedge q) \Leftrightarrow \neg p \vee \neg q $$                           |
| L3         |    Commutative Law     | $$ p \vee q \Leftrightarrow q \vee p $$  $$ p \wedge q \Leftrightarrow q \wedge p $$                                                             |
| L4         |    Assosiative Law     | $$ p \vee (q \vee r) \Leftrightarrow (p \vee q) \vee r  $$  $$ p \vee (q \wedge r) \Leftrightarrow (p \vee q) \wedge r $$                        |
| L5         |    Distributive Law    | $$ p \vee (q \wedge r) \Leftrightarrow (p \vee q) \wedge (p \vee r) $$  $$ p \wedge (q \vee r) \Leftrightarrow (p \wedge q) \vee (p \wedge r) $$ |
| L6         |     Idempotent Law     | $$ p \vee p \Leftrightarrow p $$  $$ p \wedge p \Leftrightarrow p $$                                                                             |
| L7         |      Identity Law      | $$ p \vee F_0 \Leftrightarrow p $$  $$ p \wedge T_0 \Leftrightarrow p $$                                                                         |
| L8         |      Inverse Law       | $$ p \vee \neg p \Leftrightarrow T_0 $$  $$ p \wedge \neg p \Leftrightarrow F_0 $$                                                               |
| L9         |     Domination Law     | $$ p \vee T_0 \Leftrightarrow T_0 $$  $$ p \wedge F_0 \Leftrightarrow F_0 $$                                                                     |
| L10        |     Absorption Law     | $$ p \vee (p \wedge q) \Leftrightarrow p $$  $$ p \wedge (p \vee q) \Leftrightarrow p $$                                                         |
| L11        |           -            | $$ p \iff q \Leftrightarrow (p \Rightarrow q) \wedge (q \Rightarrow p)  $$                                                                       |
| L12        |           -            | $$ p \Rightarrow q \Leftrightarrow \neg p \vee q $$                                                                                              |
| L13        |           -            | $$ p \Rightarrow q \Leftrightarrow \neg q \Rightarrow \neg p $$                                                                                  |
